partial/LambdaStack.v
@@ -67,7 +67,6 @@ Inductive Code : Set :=
 | RET : Code
 | APP : adr -> Code -> Code
 | ABS : Code -> Code -> Code
-| POP : Code -> Code
 | HALT : Code.
 
 Fixpoint comp' (e : Expr) (r : adr) (c : Code) : Code :=
@@ -75,7 +74,7 @@ Fixpoint comp' (e : Expr) (r : adr) (c : Code) : Code :=
     | Val n => LOAD n c
     | Add x y => comp' x r (STORE r (comp' y (next r) (ADD r c)))
     | Var i => LOOKUP i c
-    | App x y => comp' x r (STORE r (comp' y (next r) (APP r (POP c))))
+    | App x y => comp' x r (STORE r (comp' y (next r) (APP r c)))
     | Abs x => ABS (comp' x (next adr0) RET) c
   end.
 
@@ -106,13 +105,12 @@ Notation "⟨ c , a , e , k , s ⟩" := (conf c a e k s).
 Reserved Notation "x ==> y" (at level 80, no associativity).
 Inductive VM : Conf -> Conf -> Prop :=
  | vm_push n c s a e k :  ⟨LOAD n c, a, e, k, s⟩ ==> ⟨c, Num' n, e, k, s⟩
- | vm_pop c s s' a e k :  ⟨POP c, a, e, s' :: k, s⟩ ==> ⟨c, a, e, k, s'⟩
  | vm_add c m n r s e k : s[r] = VAL (Num' m) -> ⟨ADD r c, Num' n, e, k, s⟩
                                                  ==> ⟨c, Num'(m + n), e, k, s⟩
  | vm_store c v r s e k : ⟨STORE r c, v, e, k, s⟩
                         ==> ⟨c, v, e, k, s[r:=VAL v]⟩
  | vm_lookup e i c v a s k : nth e i = Some v -> ⟨LOOKUP i c, a, e, k, s⟩ ==> ⟨c, v, e, k, s⟩
- | vm_env a c e e' s k : s[adr0] = CLO c e -> ⟨RET, a, e', k, s⟩ ==> ⟨c, a, e, k, s⟩
+ | vm_env a c e e' s s' k : s[adr0] = CLO c e -> ⟨RET, a, e', s' :: k, s⟩ ==> ⟨c, a, e, k, s'⟩
  | vm_app c c' e e' v r s k :
      s[r]=VAL (Clo' c' e') ->
      ⟨APP r c, v, e, k,s⟩ ==> ⟨c', Num' 0, v :: e', s :: k, empty[adr0:=CLO c e]⟩
@@ -250,26 +248,24 @@ Proof.
 
   begin
     ⟨c, conv x'', convE e, k, s ⟩.
-  <== { apply vm_pop }
-    ⟨POP c, conv x'', convE e, s :: k, empty[adr0:=CLO (POP c) (convE e)] ⟩.
   <== { apply vm_env }
-    ⟨RET, conv x'', convE (y' :: e'), s :: k, empty[adr0:=CLO (POP c) (convE e)]⟩.
+    ⟨RET, conv x'', convE (y' :: e'), s :: k, empty[adr0:=CLO c (convE e)]⟩.
   <|= {apply  IHE3}
-      ⟨comp' x' (next adr0) RET, Num' 0, convE (y' :: e'), s :: k, empty[adr0:=CLO (POP c) (convE e)]⟩.
+      ⟨comp' x' (next adr0) RET, Num' 0, convE (y' :: e'), s :: k, empty[adr0:=CLO c (convE e)]⟩.
   = {auto}
-      ⟨comp' x' (next adr0) RET, Num' 0, conv y' :: convE e', s::k, empty[adr0:=CLO (POP c) (convE e)]⟩.
+      ⟨comp' x' (next adr0) RET, Num' 0, conv y' :: convE e', s::k, empty[adr0:=CLO c (convE e)]⟩.
   ≤ {auto with memory}
-      ⟨comp' x' (next adr0) RET, Num' 0, conv y' :: convE e', s[r:=VAL (Clo' (comp' x' (next adr0) RET) (convE e'))]::k, empty[adr0:=CLO (POP c) (convE e)]⟩.
+      ⟨comp' x' (next adr0) RET, Num' 0, conv y' :: convE e', s[r:=VAL (Clo' (comp' x' (next adr0) RET) (convE e'))]::k, empty[adr0:=CLO c (convE e)]⟩.
   <== {apply_eq vm_app}
-      ⟨APP r (POP c), conv y', convE e, k, s[r:=VAL (Clo' (comp' x' (next adr0) RET) (convE e'))]⟩.
+      ⟨APP r c, conv y', convE e, k, s[r:=VAL (Clo' (comp' x' (next adr0) RET) (convE e'))]⟩.
   <|= {apply IHE2}
-      ⟨comp' y (next r) (APP r (POP c)), (Clo' (comp' x' (next adr0) RET) (convE e')), convE e, k, s[r:=VAL (Clo' (comp' x' (next adr0) RET) (convE e'))]⟩.
+      ⟨comp' y (next r) (APP r c), (Clo' (comp' x' (next adr0) RET) (convE e')), convE e, k, s[r:=VAL (Clo' (comp' x' (next adr0) RET) (convE e'))]⟩.
   <== { apply vm_store }
-    ⟨STORE r (comp' y (next r) (APP r (POP c))), (Clo' (comp' x' (next adr0) RET) (convE e')), convE e, k, s⟩.
+    ⟨STORE r (comp' y (next r) (APP r c)), (Clo' (comp' x' (next adr0) RET) (convE e')), convE e, k, s⟩.
   = {auto}
-    ⟨STORE r (comp' y (next r) (APP r (POP c))), conv (Clo x' e'), convE e, k, s ⟩.
+    ⟨STORE r (comp' y (next r) (APP r c)), conv (Clo x' e'), convE e, k, s ⟩.
   <|= { apply IHE1 }
-    ⟨comp' x r (STORE r (comp' y (next r) (APP r (POP c)))), a, convE e,k, s ⟩.
+    ⟨comp' x r (STORE r (comp' y (next r) (APP r c))), a, convE e,k, s ⟩.
   [].
 Qed.
   
